wip

formal-verification/FormalVerification/SemanticEquivalence.lean
@@ -12,9 +12,11 @@ variable [Fact (Nat.Prime Order)]
 
 abbrev D := 3 -- Tree depth
 abbrev B := 2 -- Batch sizes
-abbrev gVerifyProof := SemaphoreMTB.VerifyProof_4_3
-abbrev gDeletionRound := SemaphoreMTB.DeletionRound_3_3
-abbrev gDeletionProof := SemaphoreMTB.DeletionProof_2_2_3_2_2_3
+open SemaphoreMTB renaming VerifyProof_4_3 → gVerifyProof
+open SemaphoreMTB renaming DeletionRound_3_3 → gDeletionRound
+open SemaphoreMTB renaming DeletionProof_2_2_3_2_2_3 → gDeletionProof
+open SemaphoreMTB renaming InsertionRound_3_3 → gInsertionRound
+open SemaphoreMTB renaming InsertionProof_2_3_2_2_3 → gInsertionProof
 
 def poseidon₂ : Hash F 2 := fun a => (Poseidon.perm Constants.x5_254_3 vec![0, a.get 0, a.get 1]).get 0
 
@@ -95,88 +97,83 @@ lemma VerifyProof_uncps {PathIndices: Vector F D} {Siblings: Vector F (D+1)} {k 
 -- -/
 
 -- -- Helper for proving `DeletionRound_uncps`
-lemma double_prop {a b c : Prop} : (a ∧ b ∧ a ∧ c) ↔ (a ∧ b ∧ c) := by
-  simp
-  tauto
-
 lemma select_is_match {b i1 i2 out : F} : (Gates.select b i1 i2 out) ↔ match zmod_to_bit b with
-  | Bit.zero => i2 = out
-  | Bit.one => i1 = out := by sorry
+  | Bit.zero => out = i2
+  | Bit.one => out = i1 := by sorry
 
-lemma sub_zero_is_eq {a b skip : F} : (
-    Gates.is_zero (Gates.sub a b) gate_4 ∧
-    Gates.or gate_4 skip gate_5 ∧
-    Gates.eq gate_5 (1:F)) ↔ (a = b ∨ skip = 1) := by sorry
+lemma sub_zero_is_eq {a b cond : F} {k: F -> Prop}:
+    (fun gate_2 =>
+    ∃gate_3, gate_3 = Gates.sub a b ∧
+    ∃gate_4, Gates.is_zero gate_3 gate_4 ∧
+    ∃gate_5, Gates.or gate_4 skip gate_5 ∧
+    Gates.eq gate_5 (1:F) ∧
+    ∃gate_7, Gates.select cond b gate_2 gate_7 ∧
+    k gate_7) = (fun gate_2 => match zmod_to_bit cond with
+    | Bit.zero => (a = b) ∧ k gate_2 -- Update the root
+    | Bit.one => k b  -- Skip flag set, don't update the root
+  ) := by
+  simp [select_is_match]
+  sorry
 
-  -- ↔ a = b ∨ out = 1:= by
-  -- simp [Gates.sub, Gates.is_zero]
-  -- sorry
+lemma is_vector_binary_partial {d n r} (x : Vector (ZMod n) d) : is_vector_binary x → is_vector_binary (x.take r) := by sorry
 
--- lemma or_is_match {a b out : F} : (Gates.or a b out ∧ Gates.eq out (1:F)) ↔ match zmod_to_bit a with
---   | Bit.zero => b = 1
---   | Bit.one => a = 1 := by sorry
-
--- /-!
--- `DeletionRound_uncps` proves that a single round of the deletion loop corresponds to checking that
--- the result of `MerkleTree.recover_tail` matches `Root` and returns the hash of the merkle tree with empty Leaf
--- -/
---set_option trace.Debug.Meta.Tactic.simp true
+/-!
+`DeletionRound_uncps` proves that a single round of the deletion loop corresponds to checking that
+the result of `MerkleTree.recover_tail` matches `Root` and returns the hash of the merkle tree with empty Leaf
+-/
 lemma DeletionRound_uncps {Root: F} {Index: F} {Item: F} {Proof: Vector F D} {k: F -> Prop} :
   gDeletionRound Root Index Item Proof k ↔
   ∃out: Vector F (D+1), recover_binary_zmod' out = Index ∧ is_vector_binary out ∧
-  (MerkleTree.recover_tail poseidon₂ ((Dir.create_dir_vec out).take D) Proof Item - Root = 0 ∨ out.get D = 1) ∧
-  k (match zmod_to_bit (out.get D) with
-    | Bit.zero => MerkleTree.recover_tail poseidon₂ ((Dir.create_dir_vec out).take D) Proof 0 -- Update the root
-    | Bit.one => Root  -- Skip flag set, don't update the root
+  (match zmod_to_bit (out.get D) with
+    | Bit.zero => (MerkleTree.recover_tail poseidon₂ ((Dir.create_dir_vec out).take D) Proof Item = Root) ∧ k (MerkleTree.recover_tail poseidon₂ ((Dir.create_dir_vec out).take D) Proof 0) -- Update the root
+    | Bit.one => k Root  -- Skip flag set, don't update the root
   ) := by
   unfold gDeletionRound
-  -- Is there a way to automatically unfold from gDeletionRound?
-  unfold SemaphoreMTB.DeletionRound_3_3
-  simp [Gates.to_binary, Gates.sub, Gates.is_zero, Gates.or, Gates.eq]
-  --simp [VerifyProof_looped]
-  --simp [proof_rounds_uncps]
---   simp [Gates.eq]
---   simp [Gates.to_binary]
---   simp [and_assoc]
---   apply exists_congr
---   simp
---   intros
---   subst_vars
---   rename_i gate_0 h
---   simp [double_prop]
---   rw [←Vector.ofFn_get (v := gate_0)]
---   rw [←Vector.ofFn_get (v := gate_0)] at h
---   rw [←Vector.ofFn_get (v := Proof)]
---   tauto
-  sorry
+  simp only [sub_zero_is_eq]
+  simp [VerifyProof_looped, proof_rounds_uncps]
+  simp [Gates.to_binary, and_assoc]
+  apply exists_congr
+  simp
+  intros
+  subst_vars
+  rename_i gate_0 h
+  rw [←Vector.ofFn_get (v := gate_0)]
+  rw [←Vector.ofFn_get (v := gate_0)] at h
+  rw [←Vector.ofFn_get (v := Proof)]
+  rw [and_iff_right]
+  tauto
+  have : is_vector_binary (gate_0.take 3) := by
+    apply is_vector_binary_partial
+    simp at h
+    assumption
+  rw [←Vector.ofFn_get (v := gate_0)]
+  rw [←Vector.ofFn_get (v := gate_0)] at this
+  assumption
 
--- /-!
--- `deletion_rounds` rewrites `DeletionProof_4_4_30_4` using pattern matching and recursion on the batch size
--- -/
-set_option trace.Debug.Meta.Tactic.simp false
-def deletion_rounds (DeletionIndices: Vector F n) (PreRoot: F) (IdComms: Vector F n) (MerkleProofs: Vector (Vector F D) n)  (k : F -> Prop) : Prop :=
+/-!
+`deletion_rounds` rewrites `DeletionProof_4_4_30_4` using pattern matching and recursion on the batch size
+-/
+def deletion_rounds {n} (DeletionIndices: Vector F n) (PreRoot: F) (IdComms: Vector F n) (MerkleProofs: Vector (Vector F D) n) (k : F -> Prop) : Prop :=
   match n with
   | Nat.zero => k PreRoot
   | Nat.succ _ => gDeletionRound PreRoot DeletionIndices.head IdComms.head MerkleProofs.head fun next =>
     deletion_rounds DeletionIndices.tail next IdComms.tail MerkleProofs.tail k
 
--- /-!
--- `DeletionLoop` rewrites `DeletionProof_4_4_30_4` using pattern matching and recursion on the batch size through by chaining
--- calls to `MerkleTree.recover_tail`. Ultimately we show that `DeletionLoop` is formally identical to `DeletionProof_4_4_30_4`
--- -/
+/-!
+`DeletionLoop` rewrites `DeletionProof_4_4_30_4` using pattern matching and recursion on the batch size through by chaining
+calls to `MerkleTree.recover_tail`. Ultimately we show that `DeletionLoop` is formally identical to `DeletionProof_4_4_30_4`
+-/
 def DeletionLoop {n} (DeletionIndices: Vector F n) (PreRoot: F) (IdComms: Vector F n) (MerkleProofs: Vector (Vector F D) n) (k : F -> Prop) : Prop :=
   match n with
   | Nat.zero => k PreRoot
   | Nat.succ _ =>
     ∃out: Vector F (D+1), recover_binary_zmod' out = DeletionIndices.head ∧ is_vector_binary out ∧
-    (MerkleTree.recover_tail poseidon₂ ((Dir.create_dir_vec out).take D) MerkleProofs.head IdComms.head - PreRoot = 0 ∨ out.get D = 1) ∧
-    DeletionLoop DeletionIndices.tail ((match zmod_to_bit (out.get D) with
-                                        | Bit.zero => MerkleTree.recover_tail poseidon₂ ((Dir.create_dir_vec out).take D) MerkleProofs.head 0 -- Update the root
-                                        | Bit.one => PreRoot  -- Skip flag set, don't update the root
-    )) IdComms.tail MerkleProofs.tail k
+    match zmod_to_bit (out.get D) with
+      | Bit.zero => MerkleTree.recover_tail poseidon₂ ((Dir.create_dir_vec out).take D) MerkleProofs.head IdComms.head = PreRoot ∧
+        DeletionLoop DeletionIndices.tail (MerkleTree.recover_tail poseidon₂ ((Dir.create_dir_vec out).take D) MerkleProofs.head 0) IdComms.tail MerkleProofs.tail k -- Update the root
+      | Bit.one => DeletionLoop DeletionIndices.tail PreRoot IdComms.tail MerkleProofs.tail k  -- Skip flag set, don't update the root
 
-lemma deletion_rounds_uncps {n}
-  {DeletionIndices: Vector F n} {PreRoot: F} {IdComms: Vector F n} {MerkleProofs: Vector (Vector F D) n} {k : F -> Prop}:
+lemma deletion_rounds_uncps {n} {DeletionIndices: Vector F n} {PreRoot: F} {IdComms: Vector F n} {MerkleProofs: Vector (Vector F D) n} {k : F -> Prop}:
   deletion_rounds DeletionIndices PreRoot IdComms MerkleProofs k ↔
   DeletionLoop DeletionIndices PreRoot IdComms MerkleProofs k := by
   induction DeletionIndices, IdComms, MerkleProofs using Vector.inductionOn₃ generalizing PreRoot with
@@ -191,7 +188,6 @@ lemma deletion_rounds_uncps {n}
     rename_i ih
     simp [ih]
 
--- set_option maxHeartbeats 2000000000
 lemma DeletionProof_looped (DeletionIndices: Vector F B) (PreRoot: F) (IdComms: Vector F B) (MerkleProofs: Vector (Vector F D) B) (k: F -> Prop) :
     gDeletionProof DeletionIndices PreRoot IdComms MerkleProofs k =
       deletion_rounds DeletionIndices PreRoot IdComms MerkleProofs k := by
@@ -202,10 +198,75 @@ lemma DeletionProof_looped (DeletionIndices: Vector F B) (PreRoot: F) (IdComms: 
         rw [←Vector.ofFn_get (v := MerkleProofs)]
         rfl
 
--- /-!
--- `DeletionProof_uncps` is the key lemma which shows that `DeletionProof_4_4_30_4` and `DeletionLoop` are equivalent
--- -/
+/-!
+`DeletionProof_uncps` is the key lemma which shows that `DeletionProof_4_4_30_4` and `DeletionLoop` are equivalent
+-/
 lemma DeletionProof_uncps {DeletionIndices: Vector F B} {PreRoot: F} {IdComms: Vector F B} {MerkleProofs: Vector (Vector F D) B} {k: F -> Prop}:
     gDeletionProof DeletionIndices PreRoot IdComms MerkleProofs k ↔
     DeletionLoop DeletionIndices PreRoot IdComms MerkleProofs k := by
     simp only [DeletionProof_looped, deletion_rounds_uncps]
+
+lemma double_prop {a b c d : Prop} : (b ∧ a ∧ c ∧ a ∧ d) ↔ (b ∧ a ∧ c ∧ d) := by
+  simp
+  tauto
+
+lemma InsertionRound_uncps {Index: F} {Item: F} {PrevRoot: F} {Proof: Vector F D} {k: F -> Prop} :
+  gInsertionRound Index Item PrevRoot Proof k ↔
+  ∃out: Vector F D, recover_binary_zmod' out = Index ∧ is_vector_binary out ∧
+  (MerkleTree.recover_tail poseidon₂ (Dir.create_dir_vec out) Proof 0 = PrevRoot) ∧
+  k (MerkleTree.recover_tail poseidon₂ (Dir.create_dir_vec out) Proof Item) := by
+  simp [gInsertionRound]
+  simp [Gates.to_binary, Gates.eq]
+  simp [VerifyProof_looped, proof_rounds_uncps]
+  simp [and_assoc]
+  apply exists_congr
+  intros
+  simp [double_prop]
+  rename_i gate
+  rw [←Vector.ofFn_get (v := gate)]
+  rw [←Vector.ofFn_get (v := Proof)]
+  tauto
+
+def insertion_rounds {n} (StartIndex: F) (PreRoot: F) (IdComms: Vector F n) (MerkleProofs: Vector (Vector F D) n) (k : F -> Prop) : Prop :=
+  match n with
+  | Nat.zero => k PreRoot
+  | Nat.succ _ => gInsertionRound StartIndex IdComms.head PreRoot MerkleProofs.head fun next =>
+    insertion_rounds (StartIndex + 1) next IdComms.tail MerkleProofs.tail k
+
+def InsertionLoop {n} (StartIndex: F) (PreRoot: F) (IdComms: Vector F n) (MerkleProofs: Vector (Vector F D) n) (k : F -> Prop) : Prop :=
+  match n with
+  | Nat.zero => k PreRoot
+  | Nat.succ _ =>
+    ∃out: Vector F D, recover_binary_zmod' out = StartIndex ∧ is_vector_binary out ∧
+    MerkleTree.recover_tail poseidon₂ (Dir.create_dir_vec out) MerkleProofs.head 0 = PreRoot ∧
+    InsertionLoop (StartIndex + 1) (MerkleTree.recover_tail poseidon₂ (Dir.create_dir_vec out) MerkleProofs.head IdComms.head) IdComms.tail MerkleProofs.tail k
+
+lemma insertion_rounds_uncps {n} {StartIndex: F} {PreRoot: F} {IdComms: Vector F n} {MerkleProofs: Vector (Vector F D) n} {k : F -> Prop}:
+  insertion_rounds StartIndex PreRoot IdComms MerkleProofs k ↔
+  InsertionLoop StartIndex PreRoot IdComms MerkleProofs k := by
+  induction IdComms, MerkleProofs using Vector.inductionOn₂ generalizing StartIndex PreRoot with
+  | nil => 
+    unfold insertion_rounds
+    unfold InsertionLoop
+    rfl
+  | cons => 
+    unfold insertion_rounds
+    unfold InsertionLoop
+    simp [InsertionRound_uncps]
+    rename_i ih
+    simp [ih]
+
+lemma InsertionProof_looped (StartIndex: F) (PreRoot: F) (IdComms: Vector F B) (MerkleProofs: Vector (Vector F D) B) (k: F -> Prop) :
+    gInsertionProof StartIndex PreRoot IdComms MerkleProofs k =
+      insertion_rounds StartIndex PreRoot IdComms MerkleProofs k := by
+        unfold gInsertionProof
+        simp [insertion_rounds]
+        simp [Gates.add]
+        rw [←Vector.ofFn_get (v := IdComms)]
+        rw [←Vector.ofFn_get (v := MerkleProofs)]
+        rfl
+
+lemma InsertionProof_uncps {StartIndex: F} {PreRoot: F} {IdComms: Vector F B} {MerkleProofs: Vector (Vector F D) B} {k: F -> Prop}:
+    gInsertionProof DeletionIndices PreRoot IdComms MerkleProofs k ↔
+    InsertionLoop DeletionIndices PreRoot IdComms MerkleProofs k := by
+    simp only [InsertionProof_looped, insertion_rounds_uncps]
